proof/invariants/Yield.v
@@ -1,0 +1,326 @@
+(*******************************************************************************)
+(*  © Université Lille 1, The Pip Development Team (2015-2017)                 *)
+(*                                                                             *)
+(*  This software is a computer program whose purpose is to run a minimal,     *)
+(*  hypervisor relying on proven properties such as memory isolation.          *)
+(*                                                                             *)
+(*  This software is governed by the CeCILL license under French law and       *)
+(*  abiding by the rules of distribution of free software.  You can  use,      *)
+(*  modify and/ or redistribute the software under the terms of the CeCILL     *)
+(*  license as circulated by CEA, CNRS and INRIA at the following URL          *)
+(*  "http://www.cecill.info".                                                  *)
+(*                                                                             *)
+(*  As a counterpart to the access to the source code and  rights to copy,     *)
+(*  modify and redistribute granted by the license, users are provided only    *)
+(*  with a limited warranty  and the software's author,  the holder of the     *)
+(*  economic rights,  and the successive licensors  have only  limited         *)
+(*  liability.                                                                 *)
+(*                                                                             *)
+(*  In this respect, the user's attention is drawn to the risks associated     *)
+(*  with loading,  using,  modifying and/or developing or reproducing the      *)
+(*  software by the user in light of its specific status of free software,     *)
+(*  that may mean  that it is complicated to manipulate,  and  that  also      *)
+(*  therefore means  that it is reserved for developers  and  experienced      *)
+(*  professionals having in-depth computer knowledge. Users are therefore      *)
+(*  encouraged to load and test the software's suitability as regards their    *)
+(*  requirements in conditions enabling the security of their systems and/or   *)
+(*  data to be ensured and,  more generally, to use and operate it in the      *)
+(*  same conditions as regards security.                                       *)
+(*                                                                             *)
+(*  The fact that you are presently reading this means that you have had       *)
+(*  knowledge of the CeCILL license and that you accept its terms.             *)
+(*******************************************************************************)
+
+(** * Summary 
+    This file contains the invariant of [yield]. 
+    We prove that this PIP service preserves the isolation property *)
+
+Require Import Model.ADT Model.Hardware Model.Lib Model.MALInternal Model.MAL Core.Services DependentTypeLemmas InternalLemmas Isolation Invariants StateLib Consistency WeakestPreconditions GetTableAddr.
+Import Omega List Bool.
+
+Lemma yield      (targetPartitionDescriptor : vaddr)
+                 (userTargetInterrupt : userValue)
+                 (userCallerContextSaveIndex : userValue)
+                 (flagsOnWake : interruptMask)
+                 (flagsOnYield : interruptMask)
+                 (interruptedContext : contextAddr) :
+(* Precondition *)
+{{fun (s : state) => partitionsIsolation s /\ 
+                     kernelDataIsolation s /\
+                     verticalSharing s /\
+                     consistency s }}
+(* fonction monadique *)
+yield targetPartitionDescriptor userTargetInterrupt userCallerContextSaveIndex flagsOnWake flagsOnYield interruptedContext
+(* Postcondition *)
+{{fun _ (s' : state) => partitionsIsolation s' /\
+                       kernelDataIsolation s' /\
+                       verticalSharing s' /\
+                       consistency s' }}.
+Proof.
+unfold yield.
+eapply bindRev.
+(** checkIndexPropertyLTB *)
+eapply weaken.
+apply Invariants.checkIndexPropertyLTB.
+simpl.
+intros. eapply H. simpl.
+intro userTargetInterruptIsValid.
+case_eq (negb userTargetInterruptIsValid).
+intro. eapply weaken. eapply ret. simpl. intros. intuition.
+rewrite Bool.negb_false_iff. intro HuserTargetInterruptIsValid. subst.
+eapply bindRev.
+(** getIndexFromUserValue *)
+eapply WP.weaken.
+eapply Invariants.getIndexFromUserValue.
+simpl.
+intros.
+split.
+rewrite Nat.ltb_lt in H.
+apply H.
+rewrite Nat.ltb_lt in H.
+destruct H.
+trivial.
+simpl.
+intro targetInterrupt.
+eapply bindRev.
+(** getCurPartition *)
+eapply weaken.
+eapply Invariants.getCurPartition.
+simpl.
+intros.
+eapply H.
+simpl. intro callerPartDesc.
+eapply bindRev.
+(** getPd *)
+eapply weaken.
+eapply Invariants.getPd.
+simpl.
+intros.
+split.
+apply H.
+  (* First Property *)
+  split.
+  unfold consistency in *.
+  intuition.
+  (* Second Property *)
+  assert (currentPartitionInPartitionsList s) as HcallerPartDescInPartList.
+  unfold consistency in H.
+  intuition.
+  destruct H. subst.
+  apply HcallerPartDescInPartList.
+intro callerPageDir.
+simpl.
+eapply bindRev.
+(** getNbLevel *)
+eapply Invariants.getNbLevel.
+simpl. intro nbL.
+(** checkIndexPropertyLTB - callerContextSaveIndexIsValid *)
+eapply bindRev.
+eapply weaken.
+apply Invariants.checkIndexPropertyLTB.
+simpl.
+intro s. intro preconditions. apply preconditions.
+simpl.
+intro callerContextSaveIndexIsValid.
+case_eq (negb callerContextSaveIndexIsValid);
+intro HcallerContextSaveIndexIsValid.
+eapply weaken. eapply ret. simpl. intuition.
+rewrite Bool.negb_false_iff in HcallerContextSaveIndexIsValid. subst.
+(** getIndexFromUserValue - callerContextSaveIndex **)
+eapply bindRev.
+eapply weaken.
+eapply Invariants.getIndexFromUserValue.
+simpl.
+intros.
+rewrite Nat.ltb_lt in H.
+split.
+apply H.
+destruct H.
+apply H0.
+intro callerContextSaveIndex.
+(** vidtVaddr - getVidtVAddr **)
+simpl.
+eapply bindRev.
+eapply weaken.
+eapply Invariants.ret.
+simpl.
+intros.
+apply H.
+simpl.
+intro vidtVAddr.
+(** getTableAddr - callerVidtLastMMUPage **)
+eapply WP.bindRev.
+eapply WP.weaken.
+apply getTableAddr.
+simpl.
+intros s H.
+split.
+destruct H.
+pattern s in H. 
+eexact H. subst.
+split. 
+intuition.
+split.
+instantiate (1:= callerPartDesc).
+intuition. 
+subst.
+unfold consistency in *. 
+unfold  currentPartitionInPartitionsList in *. 
+intuition.
+instantiate (1:= PDidx).
+split. intuition.
+assert(Hcons : consistency s) by intuition.
+assert(Hlevel : Some nbL = StateLib.getNbLevel) by intuition. 
+assert(Hcp : callerPartDesc = currentPartition s) by intuition.
+assert (H0 : nextEntryIsPP callerPartDesc PDidx callerPageDir s) by intuition.
+exists callerPageDir.
+split. intuition.
+
+unfold consistency in *.
+destruct Hcons as (Hpd & _ & _ &_  & Hpr & _). 
+unfold partitionDescriptorEntry in Hpd.
+assert (PDidx = PDidx \/ PDidx = sh1idx \/ PDidx = sh2idx \/  PDidx  = sh3idx
+\/  PDidx  = PPRidx \/  PDidx = PRidx) as Htmp 
+by auto.
+generalize (Hpd  (currentPartition s)  Hpr); clear Hpd; intros Hpd.
+generalize (Hpd PDidx Htmp); clear Hpd; intros Hpd.
+destruct Hpd as (Hidxpd & _& Hentry).
+destruct Hentry as (page1 & Hpd & Hnotnull).
+subst.
+split.
+ unfold nextEntryIsPP in *; destruct (StateLib.Index.succ PDidx);
+ [destruct (lookup (currentPartition s) i (memory s) beqPage beqIndex)
+ as [v |]; [ destruct v as [ p |v|p|v|ii] ; [ now contradict H0 | 
+ now contradict H0 | 
+ subst;assumption | now contradict H0| now contradict H0 ]  
+ |now contradict H0] | now contradict H0].
+subst. left. split;intuition.
+intro callerVidtLastMMUPage. simpl.
+(** simplify the new precondition **)     
+eapply WP.weaken.
+intros.
+Focus 2.
+intros.
+destruct H as (H0 & H1).
+assert ( (getTableAddrRoot' callerVidtLastMMUPage PDidx callerPartDesc MALInternal.vidtVAddr s /\ callerVidtLastMMUPage = defaultPage) \/
+(forall idx : index,
+StateLib.getIndexOfAddr MALInternal.vidtVAddr fstLevel = idx ->
+isPE callerVidtLastMMUPage idx s /\ getTableAddrRoot callerVidtLastMMUPage PDidx callerPartDesc MALInternal.vidtVAddr s  )).
+{ destruct H1 as [H1 |(Hi & Hi1 & H1)].
+  + left. trivial. 
+  + right. intros idx Hidx.
+    generalize (H1 idx Hidx);clear H1;intros H1.
+    destruct H1 as [(_& Hfalse) | [(_&Hfalse) | (Hpe &Htrue) ]].
+    - contradict Hfalse.
+      apply idxPDidxSh1notEq.
+    - contradict Hfalse.
+      apply idxPDidxSh2notEq.
+    - split; assumption.
+}
+assert (HP := conj H0 H).
+pattern s in HP.
+eapply HP.
+(** comparePageToNull - vidtLastMMUPageisNull **) 
+eapply WP.bindRev.
+eapply Invariants.comparePageToNull.
+intro vidtLastMMUPageisNull. simpl.
+case_eq vidtLastMMUPageisNull.
+{ intros.
+  eapply WP.weaken.
+  eapply WP.ret .
+  simpl. intros.
+  intuition. }
+intros. 
+subst.
+(** hypotheses cleanup *)
+eapply weaken.
+Focus 2.
+intros.
+destruct H as ((Hexec & Hconj) & Hlast).
+destruct Hconj as [HFalse | HTrue].
+- destruct HFalse.
+  subst.
+  rewrite Nat.eqb_refl in Hlast.
+  now contradict Hlast.
+Focus 2.
+destruct HTrue with (StateLib.getIndexOfAddr MALInternal.vidtVAddr fstLevel).
+trivial.
+apply beq_nat_false in Hlast.
+assert (Hdef:= conj (conj (conj Hexec H) H0) Hlast).
+pattern s in Hdef.
+apply Hdef.
+(** getIndexOfAddr - idxVidtInLastMMUPage *)
+eapply bindRev.
+eapply Invariants.getIndexOfAddr.
+simpl.
+intro idxVidtInLastMMUPage.
+(** readPresent - callerVidtIsPresent *)
+eapply bindRev.
+eapply weaken.
+eapply Invariants.readPresent.
+intros.
+simpl.
+split.
+apply H.
+intuition.
+subst.
+trivial.
+simpl.
+intro callerVidtIsPresent.
+(** negb callerVidtIsPresent *)
+case_eq (negb callerVidtIsPresent).
+intro callerVidtIsNotPresent.
+eapply weaken.
+eapply ret.
+simpl.
+intros.
+intuition.
+intro.
+apply negb_false_iff in H.
+subst.
+
+(** readAccessible - callerVidtIsAccessible *)
+eapply bindRev.
+eapply weaken.
+eapply Invariants.readAccessible.
+simpl.
+intros.
+split.
+apply H.
+intuition.
+subst.
+trivial.
+simpl.
+intro callerVidtIsAccessible.
+
+(** negb callerVidtIsAccessible *)
+case_eq (negb callerVidtIsAccessible).
+intro.
+eapply weaken.
+eapply ret.
+simpl.
+intros.
+intuition.
+intro.
+apply negb_false_iff in H.
+subst.
+
+(** readPhyEntry - callerVidt *)
+eapply bindRev.
+eapply weaken.
+eapply Invariants.readPhyEntry.
+simpl.
+intros.
+split.
+apply H.
+intuition.
+subst.
+trivial.
+simpl.
+
+(** compareVAddrToNull - calleePartDescVAddrIsDefault *)
+
+
+
+
+Admitted. 
